@base <https://uvdsl.solid.aifb.kit.edu/ontology/web-push#> .
@prefix rdf: <http://www.w3.org/1999/02/22-rdf-syntax-ns#> .
@prefix rdfs: <http://www.w3.org/2000/01/rdf-schema#> .
@prefix owl: <http://www.w3.org/2002/07/owl#> .
@prefix xsd: <http://www.w3.org/2001/XMLSchema#> .
@prefix dc: <http://purl.org/dc/elements/1.1/> .
@prefix as: <https://www.w3.org/ns/activitystreams#>.
@prefix push: <https://uvdsl.solid.aifb.kit.edu/ontology/web-push#> .


<https://uvdsl.solid.aifb.kit.edu/ontology/web-push#> a owl:Ontology ;
    dc:title "Solid Web Push Ontology" ;
    dc:date "2022-02-09" ;
    dc:creator <https://uvdsl.solid.aifb.kit.edu/profile/card#me> ;
    dc:description "This is an RDF vocabulary to model the Solid Web Push." .

push:vapidPublicKey a rdf:Property ;
    rdfs:isDefinedBy <https://www.rfc-editor.org/rfc/rfc8292> ;
    rdfs:label "VAPID Public Key" ;
    rdfs:comment """
In order for the push service to be able to validate the JWT, it
needs to learn the public key of the application server.  Also referred
to as the 'k' parameter, the public key parameter is defined for the 
'vapid' authentication scheme to carry this information.
The parameter includes an ECDSA public key [FIPS186] in uncompressed form [X9.62] 
that is encoded using base64url encoding [RFC7515].
                """ ;
    rdfs:domain as:Service ;
    rdfs:range xsd:base64Binary.

push:vapidPrivateKey a rdf:Property ;
    rdfs:isDefinedBy <https://datatracker.ietf.org/doc/rfc8292/> ;
    rdfs:label "VAPID Private Key" ;
    rdfs:comment """
When a push message subscription has been restricted to an application server, 
the request for push message delivery MUST include a JWT signed by the private key 
that corresponds to the public key used when creating the subscription.
The parameter includes an ECDSA public key that is encoded using base64url encoding [RFC7515].
                """ ;
    rdfs:domain as:Service ;
    rdfs:range xsd:base64Binary.

push:endpoint a rdf:Property ;
    rdfs:isDefinedBy <https://www.w3.org/TR/push-api/> ;
    rdfs:label "Push Subscription Endpoint" ;
    rdfs:comment """
The push endpoint of a PushSubscription is a URL that allows an application server 
to request delivery of a push message to a web application. A push subscription has 
an associated push endpoint. It MUST be the absolute URL exposed by the push service 
where the application server can send push messages to. 
A push endpoint MUST uniquely identify the push subscription.
                """ ;
    rdfs:domain as:Follow ;
    rdfs:range xsd:string.

push:keys a rdf:Property ;
    rdfs:isDefinedBy <https://www.w3.org/TR/push-api/> ;
    rdfs:label "Push Subscription Keys" ;
    rdfs:comment """
The keys property links the Subscription to its key values necessary for weak authentification.
                """ ;
    rdfs:domain as:Follow ;
    rdfs:range push:Keys.

push:Keys a rdfs:Class;
    rdfs:label "Push Subscription Keys" ;
    rdfs:comment """
The keys record contains an entry for each of the supported PushEncryptionKeyName entries 
to the URL-safe base64 encoded representation [RFC4648] of its value.
Keys named 'p256dh' and 'auth' MUST be supported, and their values MUST correspond to those 
necessary for the user agent to decrypt received push messages in accordance with [RFC8291].
                """ .

push:auth a rdf:Property ;
    rdfs:isDefinedBy <https://www.rfc-editor.org/rfc/rfc8291> ;
    rdfs:label "Push Subscription Authentication Value" ;
    rdfs:comment """
The auth value is used to retrieve the authentication secret.
                """ ;
    rdfs:domain push:keys ;
    rdfs:range xsd:base64Binary.

push:p256dh a rdf:Property ;
    rdfs:isDefinedBy <https://www.rfc-editor.org/rfc/rfc8291> ;
    rdfs:label "Push Subscription Authentication Value" ;
    rdfs:comment """
For each new subscription that the user agent generates for an application, 
it also generates a P-256 [FIPS186] key pair for use in ECDH.
                """ ;
    rdfs:domain as:Follow ;
    rdfs:range xsd:base64Binary.
